\documentclass{article}
\usepackage{amsmath}

\begin{document}

\section*{Easy Questions with Answers}
\begin{enumerate}
    \item \( x + 5 = 10 \) \\
          Solution: \( x = 10 - 5 = 5 \)
    \item \( 2x = 14 \) \\
          Solution: \( x = \frac{14}{2} = 7 \)
    \item \( x - 3 = 7 \) \\
          Solution: \( x = 7 + 3 = 10 \)
    \item \( 3x + 2 = 11 \) \\
          Solution: \( 3x = 11 - 2 = 9 \), \( x = \frac{9}{3} = 3 \)
    \item \( 4x - 8 = 0 \) \\
          Solution: \( 4x = 8 \), \( x = \frac{8}{4} = 2 \)
    \item \( 5 + 2x = 15 \) \\
          Solution: \( 2x = 15 - 5 = 10 \), \( x = \frac{10}{2} = 5 \)
    \item \( 6x = 18 \) \\
          Solution: \( x = \frac{18}{6} = 3 \)
    \item \( \frac{x}{4} = 3 \) \\
          Solution: \( x = 3 \times 4 = 12 \)
    \item \( 10x = 100 \) \\
          Solution: \( x = \frac{100}{10} = 10 \)
    \item \( x - 6 = -4 \) \\
          Solution: \( x = -4 + 6 = 2 \)
\end{enumerate}

\section*{Middle Level Questions with Answers}
\begin{enumerate}
    \item \( 2x + 3 = 9 \) \\
          Solution: \( 2x = 9 - 3 = 6 \), \( x = \frac{6}{2} = 3 \)
    \item \( 3x - 4 = 11 \) \\
          Solution: \( 3x = 11 + 4 = 15 \), \( x = \frac{15}{3} = 5 \)
    \item \( 5x + 2 = 22 \) \\
          Solution: \( 5x = 22 - 2 = 20 \), \( x = \frac{20}{5} = 4 \)
    \item \( 4(x - 1) = 8 \) \\
          Solution: \( 4x - 4 = 8 \), \( 4x = 12 \), \( x = \frac{12}{4} = 3 \)
    \item \( 2x + 3 = 5x - 3 \) \\
          Solution: \( 3 + 3 = 5x - 2x \), \( 6 = 3x \), \( x = \frac{6}{3} = 2 \)
    \item \( 3(x + 2) = 15 \) \\
          Solution: \( 3x + 6 = 15 \), \( 3x = 9 \), \( x = \frac{9}{3} = 3 \)
    \item \( 6x - 4 = 3x + 8 \) \\
          Solution: \( 6x - 3x = 8 + 4 \), \( 3x = 12 \), \( x = \frac{12}{3} = 4 \)
    \item \( 7x + 2 = 5x + 10 \) \\
          Solution: \( 7x - 5x = 10 - 2 \), \( 2x = 8 \), \( x = \frac{8}{2} = 4 \)
    \item \( 4x - 5 = 3x + 9 \) \\
          Solution: \( 4x - 3x = 9 + 5 \), \( x = 14 \)
    \item \( 5(x - 3) = 20 \) \\
          Solution: \( 5x - 15 = 20 \), \( 5x = 35 \), \( x = \frac{35}{5} = 7 \)
\end{enumerate}

\section*{Hard Questions with Answers}
\begin{enumerate}
    \item \( 4x + 3 - 2(x - 5) = 14 \) \\
          Solution: \( 4x + 3 - 2x + 10 = 14 \), \( 2x + 13 = 14 \), \( 2x = 1 \), \( x = \frac{1}{2} \)
    \item \( \frac{3x}{4} + 2 = 7 \) \\
          Solution: \( \frac{3x}{4} = 5 \), \( 3x = 20 \), \( x = \frac{20}{3} \)
    \item \( 2(x + 3) = x + 10 \) \\
          Solution: \( 2x + 6 = x + 10 \), \( 2x - x = 10 - 6 \), \( x = 4 \)
    \item \( 5x - (2x + 3) = 12 \) \\
          Solution: \( 5x - 2x - 3 = 12 \), \( 3x - 3 = 12 \), \( 3x = 15 \), \( x = 5 \)
    \item \( 6(x - 4) + 5x = 3(x + 2) \) \\
          Solution: \( 6x - 24 + 5x = 3x + 6 \), \( 11x - 24 = 3x + 6 \), \( 11x - 3x = 24 + 6 \), \( 8x = 30 \), \( x = \frac{30}{8} = \frac{15}{4} \)
    \item \( 4(x - 2) + 2(x + 1) = 18 \) \\
          Solution: \( 4x - 8 + 2x + 2 = 18 \), \( 6x - 6 = 18 \), \( 6x = 24 \), \( x = 4 \)
    \item \( 7x - 5 = 3(x + 2) \) \\
          Solution: \( 7x - 5 = 3x + 6 \), \( 7x - 3x = 6 + 5 \), \( 4x = 11 \), \( x = \frac{11}{4} \)
    \item \( 3(x - 1) + 4(x + 2) = 30 \) \\
          Solution: \( 3x - 3 + 4x + 8 = 30 \), \( 7x + 5 = 30 \), \( 7x = 25 \), \( x = \frac{25}{7} \)
    \item \( \frac{x}{2} - \frac{x}{3} = 1 \) \\
          Solution: \( \frac{3x}{6} - \frac{2x}{6} = 1 \), \( \frac{x}{6} = 1 \), \( x = 6 \)
    \item \( 2x - 5 + \frac{3x}{4} = 15 \) \\
          Solution: \( \frac{8x}{4} - \frac{20}{4} + \frac{3x}{4} = \frac{60}{4} \), \( \frac{11x}{4} = \frac{80}{4} \), \( 11x = 80 \), \( x = \frac{80}{11} \)
\end{enumerate}

\end{document}
